\documentclass[12pt]{article}

%% Language and font encodings
\usepackage[english]{babel}
\usepackage[utf8x]{inputenc}
\usepackage[T1]{fontenc}
\usepackage{fancyhdr}

%% Sets page size and margins
\usepackage[a4paper,top=3cm,bottom=2cm,left=3cm,right=3cm,marginparwidth=1.75cm]{geometry}

%% Packages
\usepackage{xcolor}
\usepackage[colorlinks=true, allcolors=red]{hyperref}
\usepackage{lipsum}
\usepackage{graphicx}
\usepackage{float}
\usepackage[all]{hypcap}
\usepackage{changepage}
\usepackage{amsmath}
\usepackage{amsthm}
\usepackage{amssymb}
\usepackage{xspace}
\usepackage{tikz}
\usepackage{amsmath,amsfonts,amssymb,amsthm}
\usepackage{mathtools}

%% Other
\graphicspath{{Figures/}}
\setlength\parindent{0pt}
\newcommand{\auth}{Giulia Baldini, Luis Fernandes, Agustin Vargas Toro}
\newcommand{\ass}{Assignment 6}

%% Page settings
\pagestyle{fancy}
\fancyhf{}
\rhead{\auth}
\lhead{\ass}
\rfoot{\thepage}
\newcommand{\real}{\mathbb{R}}
\newcommand{\inte}{\mathbb{Z}}
\newcommand{\liup}{\ensuremath{1}}
\newcommand{\lido}{\ensuremath{0}}
\newcommand{\liiup}{\ensuremath{\infty}}
\newcommand{\liido}{\ensuremath{1}}

\title{Foundations of Audio Signal Processing\\ \ass}
\author{\auth}

\begin{document}
	\maketitle
	\section*{Exercise 6.1}
	\textbf{a.} $\hat{f'}(\omega) = 2 \pi i \omega \hat{f}(\omega)$\\
	Using the integration by parts:
	\begin{alignat*}{2}
		u &= e^{-2\pi i \omega t}\\
		du &= -2\pi i \omega e^{-2\pi i \omega t} dt\\
		v &= f(t)\\
		dv &= f'(t) dt
	\end{alignat*}
	\begin{alignat*}{2}
		\hat{f'}(\omega) &= \int_{-\infty}^{\infty} f'(t) \cdot e^{-2\pi i \omega t} dt\\
		&= \left[f(t) \cdot e^{-2\pi i \omega t}\right]_{-\infty}^{\infty} - \int_{-\infty}^{\infty} -2\pi i \omega \cdot f(t) e^{-2\pi i \omega t} dt\\
		&= \left[f(t) \cdot e^{-2\pi i \omega t}\right]_{-\infty}^{\infty} + 2\pi i \omega  \int_{-\infty}^{\infty}  f(t) e^{-2\pi i \omega t} dt\\
	\end{alignat*}
	Since $f(t) \in L^2$ then:
	\begin{alignat*}{2}
	&= 2\pi i \omega \int_{-\infty}^{\infty} f(t) e^{-2\pi i \omega t} dt &= 2\pi i \omega \hat{f}(\omega)
	\end{alignat*}
	
	\textbf{b.} $\hat{f'}(\omega) = - 2 \pi i \hat{g}(\omega)$
	\begin{alignat*}{2}
		\hat{f'}(\omega) &= \frac{d}{d\omega} \hat{f}(\omega)\\
		&= \frac{d}{d\omega} \int_{-\infty}^{\infty} f(t) e^{-2\pi i \omega t} dt\\
		&= \int_{-\infty}^{\infty} \frac{d}{d\omega} (f(t)e^{-2\pi i \omega t})  dt\\
		&= \int_{-\infty}^{\infty} (-2\pi i t) f(t)e^{-2\pi i \omega t}  dt\\
		&= -2\pi i \int_{-\infty}^{\infty} t f(t)e^{-2\pi i \omega t}  dt\\
		&= -2\pi i \int_{-\infty}^{\infty} g(t) e^{-2\pi i \omega t}  dt &= -2\pi i \hat{g}(\omega)
	\end{alignat*}\\
	\textbf{c.}
	We first prove that each function is composed by an even and odd part:
	\begin{alignat*}{2}
		f(t) &= \frac{1}{2} (f(t) + f(t) + f(-t) - f(-t))\\
		&= \frac{1}{2} (f(t) + f(-t)) + \frac{1}{2} (f(t) - f(-t))\\
		&= f_e(t) + f_o(t)
	\end{alignat*}
	$f_e$ is even because:
	\begin{alignat*}{2}
		f_e(t) &=  f(t) + f(-t)\\
		&= f(-t) + f(t)\\
		&= f_e(-t)
	\end{alignat*}
	$f_o$ is odd because:
	\begin{alignat*}{2}
		f_o(t) &=  f(t) - f(-t)\\
		&= - (-f(t) + f(-t))\\
		&= - f_o(-t)
	\end{alignat*}
	We now prove that the integral of the product of odd and even functions is 0:
	\begin{alignat*}{2}
		\int_{-\infty}^{\infty} f_e(t) f_o(t) dt &= \int_{-\infty}^{0} f_e(t) f_o(t) dt+ \int_{0}^{\infty} f_e(t) f_o(t) dt\\
		&= \int_{0}^{\infty} f_e(-t) f_o(-t) dt+ \int_{0}^{\infty} f_e(t) f_o(t) dt\\
		&= \int_{0}^{\infty} (f_e(-t) f_o(-t) + f_e(t) f_o(t)) dt\\
		&= \int_{0}^{\infty} (f_e(-t) f_o(-t) - f_e(-t) f_o(-t)) dt &= 0
	\end{alignat*}
	Now we start proving that $Re(\hat{f})$ is even and $Re(\hat{f})$ is odd.
	\begin{alignat*}{2}
	\hat{f}(\omega) &= \int_{-\infty}^{\infty} f(t) e^{-2\pi i \omega t} dt\\
	&= \int_{-\infty}^{\infty} f(t)(\cos(2\pi\omega t) - i \sin(2\pi\omega t)) dt\\
	&= \int_{-\infty}^{\infty} f(t)(\cos(2\pi\omega t) ) - \int_{-\infty}^{\infty} f(t)(i \sin(2\pi\omega t)) dt\\
	\end{alignat*}
	Now we can substitute $f(t)$ with $f_e(t) + f_o(t)$ and we obtain:
	\begin{alignat*}{2}
		&=\int_{-\infty}^{\infty} (f_e(t) + f_o(t))(\cos(2\pi\omega t) ) - \int_{-\infty}^{\infty} (f_e(t) + f_o(t))(i \sin(2\pi\omega t)) dt\\
		&= \int_{-\infty}^{\infty} f_e(t)(\cos 2\pi\omega t) dt + \int_{-\infty}^{\infty} f_o(t)\cos(2\pi\omega t) dt -\\ 
		&\int_{-\infty}^{\infty} f_e(t)i \sin(2\pi\omega t) dt - \int_{-\infty}^{\infty} f_o(t)i \sin(2\pi\omega t) dt
	\end{alignat*}
	Since $\cos$ is an even function and $\sin$ is an odd function, then we can delete the two middle elements, since they are integrals of a product of an odd and an even function.
	\begin{alignat*}{2}
		&= \int_{-\infty}^{\infty} f_e(t)\cos(2\pi\omega t) dt - \int_{-\infty}^{\infty} f_o(t)i \sin(2\pi\omega t) dt\\
		&= \hat{f}_e(\omega) - \hat{f}_o(\omega)
	\end{alignat*}
	Since $f(t)$ is real, then $\hat{f}_e(\omega)$ is real too (because it does not contain any imaginary part) and $\hat{f}_o(\omega)$ is imaginary because it has an imaginary component.\\\\
	\textbf{d.} Assuming that $f(\omega)$ is real and even, it holds that $f(\omega) = f(-\omega)$, and for $\hat{f}$ to be even we need to prove that $\hat{f}(\omega) = \hat{f}(-\omega)$.
	\begin{alignat*}{2}
	\hat{f}(\omega) &= \int_{-\infty}^{\infty} f(t) e^{-2\pi i \omega t} dt\\
	&= \int_{-\infty}^{\infty} f(-t) e^{2\pi i \omega (-t)} dt
	\end{alignat*}
	We now substitute $-t$ with $u$:
	\begin{alignat*}{2}
	&= \int_{-\infty}^{\infty} f(u) e^{2\pi i \omega (u)} du\\
	&= \int_{-\infty}^{\infty} f(u) e^{2\pi (-i) (-\omega) (u)} du\\
	&= \int_{-\infty}^{\infty} f(u) e^{-2\pi i (-\omega) (u)} du &= \hat{f}(-\omega)
	\end{alignat*}
	We now have to prove that if $f(\omega)$ is real and even, $\hat{f}$ is real.
	\begin{alignat*}{2}
	\hat{f}(\omega) &= \int_{-\infty}^{\infty} f(t) e^{-2\pi i \omega t} dt\\
	&= \int_{-\infty}^{\infty} f(t)(\cos(2\pi\omega t) - i \sin(2\pi\omega t)) dt\\
	&= \int_{-\infty}^{\infty} f(t)(\cos(2\pi\omega t) )
	\end{alignat*}
	which is real.
	\section*{Exercise 6.2}
	
	\textbf{a.}
	
	$$\langle f | A_k \rangle = \sqrt{2}\int_{0}^{1} f(t)cos(2 \pi k t) dt$$ 
	
	$$ = \sqrt{2} \Bigg(\int_0^{1/2} -cos \left(t2 \pi k t\right)dt + \int_{1/2}^{1} cos \left(2 \pi k t\right) dt \Bigg) $$
	
	$$ = \sqrt{2} \Bigg[ \frac{-sin(2\pi k t)}{2 \pi k} \Bigg|^{1/2}_{0} + \frac{sin( 2 \pi k t}{2 \pi k} \Bigg|^{1}_{1/2} \bigg]$$
	
	$$ = \sqrt{2}\Bigg[ \frac{sin(2 \pi k)}{2 \pi k} - \frac{sin(\pi k)}{ \pi k} \Bigg]$$
	
	$$\langle f | B_k \rangle = \sqrt{2}\int_{0}^{1} f(t)sin(2 \pi k t) dt$$ 
	
	$$ = \sqrt{2} \Bigg[ \int^{1/2}_{0} -sin(2 \pi k t)dt + \int^{1}_{1/2}sin(2 \pi k)dt \Bigg] $$
	
	$$= sqrt{2} \Bigg[ \frac{cos(2 \pi k)}{2 \pi k} \Bigg|^{1/2}_{0} - \frac{cos(2 \pi k)}{2 \pi k}\Bigg|^{1}_{1/2} \Bigg]  $$
	
	$$ = \frac{\sqrt{2}}{n k} \Bigg[ \frac{cos(\pi k)}{2 \pi k} - \frac{1}{2 \pi k} - \frac{cos(2 \pi k)}{2 \pi k} + \frac{cos( \pi k) }{ 2 \pi k}  \Bigg]$$
	
	$$= \frac{\sqrt{2}}{\pi k} \Bigg[ cos(\pi k) - \frac{1}{2} - \frac{cos(2 \pi k)}{2}\Bigg]$$

	\textbf{b-c.} The solutions can be found inside the \texttt{code} folder.
\end{document}
